Refactor to separate syntax and semantics of TensorGraph

theories/GraphCore/TensorGraph.v
@@ -1,180 +1,121 @@
-From QuantumLib Require Import Complex.
-Require Import Tensor.
-From stdpp Require Import list sorting fin_maps.
-From stdpp Require Import pmap gmap.
-Require Import Aux_stdpp.
-Require Import TensorExprDBSyntax TensorExprDBSemantics.
-Require Import ZXCore.
-Require ZifyBool.
+Require Export Tensor.
+From stdpp Require Export list sorting fin_maps.
+From stdpp Require Export pmap gmap.
+Require Export Aux_stdpp.
+
+(* Basic definitions and structural operations on TensorGraphs *)
 
 
-Definition bcons (b : bool) (p : positive) : positive :=
-  match b with 
-  | true => xI p
-  | false => xO p
-  end.
+Notation edge := (prod nat nat).
 
-#[global] 
-Program Instance Op_bcons : ZifyClasses.BinOp 
-  (T1:=bool) bcons := {
-  TBOp b p := (2 * p + Z.b2z b)%Z;
+(* A labelled edge *)
+Notation labedge := (prod nat edge).
+
+(* A graph with nodes labeled by elements of [T] *)
+Record TensorGraph {T : Type} := mk_tg {
+  nodes : gmap nat T;
+  edges : list edge
 }.
-Next Obligation.
-  cbn.
-  intros [] ?; cbn; lia.
-Qed.
+#[global] Arguments TensorGraph T : clear implicits.
+#[global] Arguments mk_tg {_} (_ _) : assert.
 
-Add Zify BinOp Op_bcons.
+Definition TensorGraph2pair {T} (tg : TensorGraph T) : 
+  gmap nat T * list edge :=
+  (tg.(nodes), tg.(edges)).
 
-#[export] Instance bcons_inj2 : Inj2 (=) (=) (=) bcons.
-Proof.
-  hnf.
-  lia.
-Qed.
+#[global] Coercion TensorGraph2pair : TensorGraph >-> prod.
 
-(* Combine input and output maps to get the local variable map *)
-Definition gmaps_to_Pmap {A} 
-  (minput : gmap nat A) (moutput : gmap nat A) : Pmap A :=
-  (kmap (bcons false ∘ Pos.of_succ_nat) minput ∪ 
-      kmap (bcons true ∘ Pos.of_succ_nat) moutput).
-
-
-
-Notation TensorMap R A := 
-  (gmap nat (@DimensionlessTensor R A)).
 
 Section TensorGraph.
 
-Context {R : Type} {A : Type}.
+Context {T : Type}.
 
+Let TensorGraph := (TensorGraph T).
 
-Definition EdgeSet := list (nat * nat).
+Implicit Types tg : TensorGraph.
 
-Definition TensorGraph := 
-  (TensorMap R A * EdgeSet)%type.
+(* is_key explicitly only depends on the nodes *)
+Definition is_key (tm : gmap nat T) (n : nat) : Prop :=
+  is_Some (tm !! n).
 
-Definition is_key (tg : TensorGraph) (n : nat) : Prop :=
-  is_Some (tg.1 !! n).
+Definition is_input (tm : gmap nat T) (nm : edge) : Prop :=
+  is_key tm (fst nm).
 
-Definition is_input (tg : TensorGraph) (nm : nat * nat) : Prop :=
-  is_key tg (fst nm).
+Definition is_output (tm : gmap nat T) (nm : edge) : Prop :=
+  is_key tm (snd nm).
 
-Definition is_output (tg : TensorGraph) (nm : nat * nat) : Prop :=
-  is_key tg (snd nm).
+Definition is_internal tm (e : edge) :=
+  is_key tm (fst e) /\ is_key tm (snd e).
 
-Definition count_inputs (tg : TensorGraph) : nat := 
-  length (filter (is_input tg) (snd tg)).
+Definition not_internal tm (e : edge) :=
+  ~ is_internal tm e.
 
-Definition count_outputs (tg : TensorGraph) : nat := 
-  length (filter (is_output tg) (snd tg)).
 
 Definition inputs (tg : TensorGraph) : gset nat :=
-  filter (fun k => ~ is_key tg k) $ 
+  filter (fun k => ~ is_key tg.1 k) $
     list_to_set tg.2.*1.
 
 Definition outputs (tg : TensorGraph) : gset nat :=
-  filter (fun k => ~ is_key tg k) $ 
+  filter (fun k => ~ is_key tg.1 k) $
     list_to_set tg.2.*2.
 
 
-Definition is_internal tg (e : nat * nat) := 
-  is_key tg (fst e) /\ is_key tg (snd e).
-
-Definition not_internal tg (e : nat * nat) :=
-  ~ is_internal tg e.
 
 
-Definition internal_edges tg := 
-  filter (is_internal tg) tg.2.
+Definition internal_edges tg :=
+  filter (is_internal tg.1) tg.2.
 
 Definition external_edges tg :=
-  filter (not_internal tg) tg.2.
+  filter (not_internal tg.1) tg.2.
 
-Definition i_internal_edges tg := 
+Definition i_internal_edges tg :=
   enumerate (internal_edges tg).
 
 Definition i_external_edges tg :=
   enumerate (external_edges tg).
 
-Definition mk_internal_var (e : nat * (nat * nat)) :=
-  rel (Pos.of_succ_nat (fst e)).
+Definition is_node_input (k : nat) (e : edge) : Prop :=
+  e.2 = k.
 
-Definition mk_external_var (is_output : bool) (e : nat * (nat * nat)) :=
-  loc (bcons is_output (Pos.of_succ_nat (if is_output then e.2.2 else e.2.1))).
+#[export] Instance is_node_input_dec k e : Decision (is_node_input k e) := 
+  decide_rel _ (e.2) k.
 
-Definition mk_node (tg : TensorGraph)
-  (n : nat) : Idx * list var * list var :=
-    let is_input e := snd (snd e) = n in
-    let is_output e := fst (snd e) = n in
-    let i_internal_inputs  := filter is_input (i_internal_edges tg) in
-    let i_internal_outputs := filter is_output (i_internal_edges tg) in
-    let i_external_inputs  := filter is_input (i_external_edges tg) in
-    let i_external_outputs := filter is_output (i_external_edges tg) in
-    (Pos.of_succ_nat n, 
-      (mk_internal_var <$> i_internal_inputs) ++ 
-        (mk_external_var false <$> i_external_inputs), 
-      (mk_internal_var <$> i_internal_outputs) ++ 
-        (mk_external_var true <$> i_external_outputs)).
+Definition is_node_output (k : nat) (e : edge) : Prop :=
+  e.1 = k.
+
+#[export] Instance is_node_output_dec k e : Decision (is_node_output k e) := 
+  decide_rel _ (e.1) k.
+
+Definition node_input_edges (k : nat) (les : list labedge) : list labedge :=
+  filter (is_node_input k ∘ snd) les.
+
+Definition node_output_edges (k : nat) (les : list labedge) : list labedge :=
+  filter (is_node_output k ∘ snd) les.
 
 
 
 
-Definition add_vertex (n : nat) (t : DimensionlessTensor (R:=R) A) 
-  (tg : TensorGraph) : TensorGraph:=
-  (<[n := t]> (fst tg), snd tg).
+Definition in_arity (es : list edge) (k : nat) :=
+  length (filter (is_node_input k) es).
 
-Definition add_edge (e : nat * nat) 
+Definition out_arity (es : list edge) (k : nat) :=
+  length (filter (is_node_output k) es).
+
+
+
+
+Definition add_vertex (n : nat) (t : T)
   (tg : TensorGraph) : TensorGraph :=
-  (fst tg, e :: snd tg).
+  mk_tg (<[n := t]> tg.1) tg.2.
 
-Definition empty_graph : TensorGraph := (∅, []).
+Definition add_edge (e : edge)
+  (tg : TensorGraph) : TensorGraph :=
+  mk_tg tg.1 (e :: tg.2).
 
-
-
-
-Definition graph_tensorlist_semantics (tg : TensorGraph) : tensorlist :=
-  mk_tl (const 0%nat <$> internal_edges tg) 
-    (mk_node tg <$> (map_to_list (fst tg)).*1).
-
-Definition graph_V : nat -> Type := fun _ => A.
-Definition graph_Vsum `{Summable A} : forall k, Summable (graph_V k) 
-  := fun _ => _.
+Definition empty_graph : TensorGraph := mk_tg ∅ [].
 
 
 
-(* Combine input and output maps to get the local variable map *)
-Definition graph_ml (minput : gmap nat A) (moutput : gmap nat A) : 
-  Pmap (Vval graph_V) :=
-  @mk_Vval graph_V 0 <$> gmaps_to_Pmap minput moutput. 
-
-Fixpoint graph_tensor_to_V_n_args_aux {n} : forall (t : vec A n -> R),
-  V_n_args graph_V (replicate n 0) R :=
-  match n with
-  | O => fun t => t [#]
-  | S n' => fun t => 
-    fun a => graph_tensor_to_V_n_args_aux (t ∘ vcons a)
-  end.
-
-Definition graph_tensor_to_V_n_args {n m} (t : vec A n -> vec A m -> R) :=
-  graph_tensor_to_V_n_args_aux (uncurry t ∘ Vector.splitat n).
-
-Definition graph_mabs (tg : TensorGraph) : Pmap (@Vfunc R graph_V) :=
-  kmap (Pos.of_succ_nat) $ map_imap (fun n (dt : DimensionlessTensor A) => 
-    let node := mk_node tg n in 
-    let inarity := length node.1.2 in 
-    let outarity := length node.2 in 
-    Some $ mk_Vfunc graph_V (replicate (inarity + outarity) 0)
-      (graph_tensor_to_V_n_args (dt inarity outarity))
-    ) tg.1.
-
-Definition graph_map_semantics `{SR : SemiRing R rO rI radd rmul req} `{!Summable A} 
-  (tg : TensorGraph) 
-  (minput : gmap nat A) (moutput : gmap nat A) : R :=
-  tl_total_semantics (SR:=SR) graph_V (Vsum:=graph_Vsum)
-    (graph_mabs tg)
-    ∅
-    (graph_ml minput moutput)
-    (graph_tensorlist_semantics tg).
 
 Definition graph_insize (tg : TensorGraph) : nat := size (inputs tg).
 Definition graph_outsize (tg : TensorGraph) : nat := size (outputs tg).
@@ -186,16 +127,6 @@ Definition sorted_inputs (tg : TensorGraph) : list nat :=
 Definition sorted_outputs (tg : TensorGraph) : list nat :=
   merge_sort le $ elements (outputs tg).
 
-
-Definition graph_list_semantics `{SR : SemiRing R rO rI radd rmul req} `{!Summable A} 
-  (tg : TensorGraph) (ins : list A) (outs : list A) : R :=
-  graph_map_semantics tg 
-    (list_to_map $ zip (sorted_inputs tg) ins)
-    (list_to_map $ zip (sorted_outputs tg) outs).
-
-Definition graph_vector_semantics `{SR : SemiRing R rO rI radd rmul req} `{!Summable A} 
-  (tg : TensorGraph) (ins : vec A (graph_insize tg)) (outs : vec A (graph_outsize tg)) : R :=
-  graph_list_semantics tg (vec_to_list ins) (vec_to_list outs).
 
 End TensorGraph.
 
@@ -210,85 +141,3 @@ Notation "∅G" := empty_graph : graph_scope.
 Open Scope graph_scope.
 Open Scope nat.
 
-Definition example_graph : TensorGraph (R:=C) (A:=bool) := 
-  ∅G +[ 1 := (fun n m => @zsp n m 0) ]
-     +[ 3 := (fun n m => @zsp n m 0) ]
-     +{ (1,2) ; (1,3) ; (1,2) ; (1,3) ; (1,4) }.
-
-
-Definition example_graph' : TensorGraph (R:=C) (A:=bool) := 
-  ∅G +[ 1 := (fun n m => @zsp n m 0) ]
-     +[ 3 := (fun n m => @zsp n m 0) ]
-     +{ (1,2) ; (1,3) ; (3,4) }.
-
-Compute graph_tensorlist_semantics example_graph.
-
-Compute elements $ inputs example_graph.
-
-Compute elements $ outputs example_graph.
-
-Compute graph_tensorlist_semantics example_graph'.
-
-Compute elements $ inputs example_graph'.
-
-Compute elements $ outputs example_graph'.
-
-
-(* 
-From VyZX Require Import CoreData.
-
-Open Scope ZX_scope.
-
-Open Scope nat_scope.
-
-Example example_graph'_map_semantics : forall b b',
-  graph_map_semantics example_graph' 
-    ∅ {[2:=b; 4:=b']} = 
-  ⟦ Z 0 2 0 ⟷ (— ↕ Z 1 1 0) ⟧
-    (Bits.funbool_to_nat 2 ([b;b'] !!!.)) O.
-Proof.
-  cbn -[graph_map_semantics].
-  unfold kron.
-  cbn -[graph_map_semantics].
-  intros [] []; cbn -[graph_map_semantics]; (etransitivity; 
-    [unfold example_graph'; 
-      remember @zsp as zsp' eqn:Hzsp; 
-      vm_compute|Csimpl; reflexivity]);
-  subst zsp'; cbn -[Cexp]; 
-  change R0 with 0%R; rewrite ?Cexp_0; lca.
-Qed.
-
-Example example_graph'_list_semantics : forall b b',
-  graph_list_semantics example_graph' 
-    [] [b; b'] = 
-  ⟦ Z 0 2 0 ⟷ (— ↕ Z 1 1 0) ⟧
-    (Bits.funbool_to_nat 2 ([b;b'] !!!.)) O.
-Proof.
-  cbn -[graph_list_semantics].
-  unfold kron.
-  cbn -[graph_list_semantics].
-  intros [] []; cbn -[graph_list_semantics]; (etransitivity; 
-    [unfold example_graph'; 
-      remember @zsp as zsp' eqn:Hzsp; 
-      vm_compute|Csimpl; reflexivity]);
-  subst zsp'; cbn -[Cexp]; 
-  change R0 with 0%R; rewrite ?Cexp_0; lca.
-Qed.
-
-Example example_graph'_vector_semantics : forall b b',
-  graph_vector_semantics example_graph' 
-    [# ] [# b; b'] = 
-  ⟦ Z 0 2 0 ⟷ (— ↕ Z 1 1 0) ⟧
-    (Bits.funbool_to_nat 2 ([b;b'] !!!.)) O.
-Proof.
-  cbn -[graph_vector_semantics].
-  unfold kron.
-  cbn -[graph_vector_semantics].
-  intros [] []; cbn -[graph_vector_semantics]; (etransitivity; 
-    [unfold example_graph'; 
-      remember @zsp as zsp' eqn:Hzsp; 
-      vm_compute|Csimpl; reflexivity]);
-  subst zsp'; cbn -[Cexp]; 
-  change R0 with 0%R; rewrite ?Cexp_0; lca.
-Qed.
- *)
