theories/GraphCore/TensorGraphFacts.v
@@ -11,113 +11,6 @@ Require Import TensorGraph.
 #[local] Coercion pos_to_nat_pred : positive >-> nat.
 
 (* FIXME: Move *)
-Lemma Forall_filter {A} (P Q : A -> Prop) `{HP : forall a, Decision (P a)}
-  (l : list A) :
-  Forall Q (filter P l) <-> Forall (fun a => P a -> Q a) l.
-Proof.
-  induction l; [now split; constructor|].
-  cbn.
-  case_decide as HPa.
-  - rewrite 2 Forall_cons, IHl. tauto.
-  - rewrite Forall_cons, IHl. tauto.
-Qed.
-
-Lemma fmap_const {A B} (l : list A) (b : B) :
-  const b <$> l = replicate (length l) b.
-Proof.
-  induction l; cbn; f_equal; assumption.
-Qed.
-
-Lemma lookup_gmaps_to_Pmap {A} (mi mo : gmap nat A) p :
-  gmaps_to_Pmap mi mo !! p =
-  match p with
-  | xH => None
-  | p~0 => mi !! (p:>nat)
-  | p~1 => mo !! (p:>nat)
-  end.
-Proof.
-  unfold gmaps_to_Pmap.
-  rewrite lookup_union.
-  destruct p.
-  - rewrite (lookup_kmap_None _ _ _).2 by now cbn; lia.
-    rewrite option_union_left_id.
-    replace p~1 with ((bcons true ∘ Pos.of_succ_nat) p) by now cbn; lia.
-    rewrite lookup_kmap by apply _.
-    reflexivity.
-  - replace p~0 with ((bcons false ∘ Pos.of_succ_nat) p) by now cbn; lia.
-    rewrite lookup_kmap by apply _.
-    rewrite (lookup_kmap_None _ _ _).2 by now cbn; lia.
-    rewrite option_union_right_id.
-    reflexivity.
-  - rewrite 2 (lookup_kmap_None _ _ _).2 by now cbn; lia.
-    reflexivity.
-Qed.
-
-Lemma length_list_filter_ext {A B} (P : A -> Prop) (Q : B -> Prop)
-  `{HP : forall a, Decision (P a)} `{HQ : forall b, Decision (Q b)}
-  (l : list A) (l' : list B) :
-  Forall2 (λ a b, P a <-> Q b) l l' ->
-  length (filter P l) = length (filter Q l').
-Proof.
-  intros Hall.
-  induction Hall; [reflexivity|].
-  cbn.
-  unshelve (erewrite decide_ext by eassumption); [auto|].
-  case_decide; cbn; f_equal; easy.
-Qed.
-
-(* FIXME: Move *)
-Lemma lengthN_fmap {A B} (f : A -> B) (l : list A) :
-  lengthN (f <$> l) = lengthN l.
-Proof.
-  apply lengthN_eq, length_fmap.
-Qed.
-Lemma ppermute_fmap {A B} p (f : A -> B) (l : list A) :
-  ppermute p (f <$> l) = f <$> ppermute p l.
-Proof.
-  destruct (ppermute_case p l) as [(Hbdd & Hsome) | (Hndbb & Hnone)].
-  - apply (list_eq_same_length _ _ _ eq_refl);
-    [now rewrite length_fmap, 2 length_ppermute, length_fmap|].
-    intros i x y.
-    rewrite length_fmap, length_ppermute.
-    intros Hi.
-    rewrite lookup_ppermute_alt_bdd by now rewrite ?lengthN_fmap, ?length_fmap.
-    rewrite 2 list_lookup_fmap.
-    rewrite lookup_ppermute_alt_bdd by easy.
-    congruence.
-  - now rewrite 2 ppermute_not_bdd by now rewrite ?lengthN_fmap.
-Qed.
-Lemma default_is_Some_ext_mor_gen {B} {R : relation B} (d d' : B)
-  (mb mb' : option B) : R d d' ->
-  (forall b, mb = Some b -> mb' = None -> R b d') ->
-  (forall b', mb = None -> mb' = Some b' -> R d b') ->
-  (forall b b', mb = Some b -> mb' = Some b' -> R b b') ->
-  R (default d mb) (default d' mb').
-Proof.
-  destruct mb, mb'; cbn; eauto.
-Qed.
-Lemma default_is_Some_ext_mor {B} {R : relation B} (d d' : B)
-  (mb mb' : option B) :
-  (is_Some mb <-> is_Some mb') ->
-  R d d' ->
-  (forall b b', mb = Some b -> mb' = Some b' -> R b b') ->
-  R (default d mb) (default d' mb').
-Proof.
-  intros HSome Hd HR.
-  rewrite 2 is_Some_alt in HSome.
-  destruct mb, mb'; cbn; naive_solver.
-Qed.
-Lemma not_elem_of_list_fmap {A B} (f : A -> B) (l : list A) (b : B) :
-  b ∉ f <$> l <-> forall a, a ∈ l -> f a ≠ b.
-Proof.
-  rewrite elem_of_list_fmap.
-  naive_solver.
-Qed.
-Lemma Permutation_swap_app_app {A} (l1 l2 l3 l4 : list A) :
-  (l1 ++ l2) ++ (l3 ++ l4) ≡ₚ (l1 ++ l3) ++ (l2 ++ l4).
-Proof.
-  solve_Permutation.
-Qed.
 Lemma forall_var (P : var -> Prop) :
   (forall v, P v) <-> (forall r, P (rel r)) /\ (forall l, P (loc l)) /\
     (forall g, P (glob g)).
@@ -125,31 +18,11 @@ Proof.
   split; [auto|].
   now intros (?&?&?) [].
 Qed.
-Lemma and_is_True_r {P Q} : Q -> P /\ Q <-> P.
-Proof. tauto. Qed.
-Lemma and_is_True_l {P Q} : P -> P /\ Q <-> Q.
-Proof. tauto. Qed.
-Lemma and_or_distr_r {P Q R} : (P \/ Q) /\ R <-> P /\ R \/ Q /\ R.
-Proof. tauto. Qed.
-Lemma and_or_distr_l {P Q R} : P /\ (Q \/ R) <-> P /\ Q \/ P /\ R.
-Proof. tauto. Qed.
-Lemma iff_True {P} : (P <-> True) <-> P.
-Proof. tauto. Qed.
-Lemma iff_True_1 {P} : P -> (P <-> True).
-Proof. tauto. Qed.
-Lemma iff_True_2 {P} : (P <-> True) -> P.
-Proof. tauto. Qed.
 
 
 
 
-
-
-
-Definition mk_tg {R A} (tm : TensorMap R A) (es : EdgeSet) : TensorGraph :=
-  (tm, es).
-
-
+(* 
 Section TensorGraphFacts.
 
 Context {R : Type} {A : Type}.
@@ -820,4 +693,4 @@ Proof.
 
 *)
 
-End TensorGraphFacts.
+End TensorGraphFacts. *)
