theories/GraphCore/TensorGraphExpr.v
@@ -1,0 +1,45 @@
+Require Export TensorGraph Aux_pos.
+
+Require Export TensorExprDBSyntax.
+
+(* Semantics of TensorGraphs into tensor expressions *)
+
+
+Section TensorGraphExpr.
+
+Context {T : Type}.
+
+Let TensorGraph := (TensorGraph T).
+
+Implicit Types tg : TensorGraph.
+
+Definition input_edges (linternal lexternal : list labedge) 
+  (k : nat) : list var :=
+  ((rel ∘ Pos.of_succ_nat ∘ fst) <$> 
+    node_input_edges k linternal) ++
+  ((loc ∘ bcons false ∘ Pos.of_succ_nat ∘ fst) <$> 
+    node_input_edges k lexternal).
+
+Definition output_edges (linternal lexternal : list labedge) 
+  (k : nat) : list var :=
+  ((rel ∘ Pos.of_succ_nat ∘ fst) <$> 
+    node_output_edges k linternal) ++
+  ((loc ∘ bcons false ∘ Pos.of_succ_nat ∘ fst) <$> 
+    node_output_edges k lexternal).
+
+
+
+Definition mk_node (linternal lexternal : list labedge)
+  (k : nat) :=
+  (Pos.of_succ_nat k, input_edges linternal lexternal k,
+    output_edges linternal lexternal k).
+
+
+
+
+Definition graph_tensorlist_semantics (tg : TensorGraph) : tensorlist :=
+  mk_tl (const 0%nat <$> internal_edges tg)
+    (mk_node (i_internal_edges tg) (i_external_edges tg) <$> 
+      (map_to_list (fst tg)).*1).
+
+End TensorGraphExpr.
