theories/GraphCore/ZXGraph.v
@@ -1,0 +1,106 @@
+Require Import ZXCore.
+From QuantumLib Require Import Complex.
+Require Import TensorGraphSemantics.
+Open Scope nat_scope.
+
+Notation "'ZXG'" := (TensorGraph (bool * R)) (at level 0).
+
+(* Check ZXG. *)
+
+Instance ZXCALC : TensorLike C bool (bool * R) := {
+  interpretTensor (x : bool * R) := match x with
+  | (true, r)  => fun n m => @zsp n m r
+  | (false, r) => fun n m => @zsp n m r
+  end
+}.
+
+Definition example_graph : TensorGraph (bool*R) := 
+  ∅G +[ 1 := (true, 0%R) ]
+     +[ 3 := (true, 0%R) ]
+     +{ (6, 1) ; (5, 1) ; (1,2) ; (1,3) ; (1,2) ; (1,3) ; (1,4) }.
+
+
+(* TODO: Rework these and put them in TensorGraph *)
+
+Definition relabel_vertex {T} (n m : nat) (tg : TensorGraph T) : TensorGraph T :=
+  let '(mk_tg verts edges) := tg in
+  let verts' := 
+    match lookup n verts with
+    | Some t => <[m := t]> (delete n verts)
+    | None => verts
+    end in
+  let relabel_idx i := if i =? n then m else i in
+  let edges' := (fun e : (nat * nat) => 
+    let (s, d) := e in (relabel_idx s, relabel_idx d)) <$> edges in
+  mk_tg verts' edges'.
+
+
+Definition has_edge (n m : nat) (es : list edge) : Prop :=
+  (n, m) ∈ es \/ (m, n) ∈ es.
+
+Definition connected {T} (n m : nat) (tg : TensorGraph T) : Prop :=
+  is_key tg.1 n /\ is_key tg.1 m /\ has_edge n m tg.2.
+
+Definition remove_vertex {T} (n : nat) (tg : TensorGraph T) : TensorGraph T :=
+  let '(mk_tg verts edges) := tg in
+  let verts' := delete n verts in
+  let edges' := 
+    filter (fun e : (nat * nat) => let (s, d) := e in negb ((s =? n) || (d =? n))) edges in
+  mk_tg verts' edges'.
+
+Definition remove_edge {T} (n m : nat) (tg : TensorGraph T) : TensorGraph T:=
+  let '(mk_tg verts edges) := tg in
+  let edges' := filter (fun e : (nat * nat) => let (s, d) := e in ((s =? n) && (d =? m) || (s =? m) && (d =? n))) edges in
+  mk_tg verts edges'.
+
+Definition successors {T} (n : nat) (tg : TensorGraph T) : list nat :=
+  map snd (filter (fun e => fst e =? n) (snd tg)).
+
+Definition predecessors {T}(n : nat) (tg : TensorGraph T) : list nat :=
+  map fst (filter (fun e => snd e =? n) (snd tg)).
+
+Fixpoint add_edges {T} (es : list (nat * nat)) 
+  (tg : TensorGraph T) :=
+  match es with
+  | [] => tg
+  | e :: es' => add_edge e (add_edges es' tg)
+  end.
+
+
+Definition rotation (n : nat) (zxg : ZXG) : option R :=
+  snd <$> (zxg.1 !! n).
+
+Definition vertex_type (n : nat) (zxg : ZXG) : option bool :=
+  fst <$> (zxg.1 !! n).
+
+Definition hopf (n m : nat) (zxg : ZXG) : ZXG :=
+  remove_edge n m (remove_edge n m zxg).
+
+Definition option_eqb_bool (a : option bool) (b : option bool) : bool :=
+  match a with
+  | Some x => match b with
+              | Some y => eqb x y
+              | None => false
+              end
+  | None => false
+  end.
+
+Definition fuse (n m : nat) (zxg : ZXG) : ZXG :=
+  let preds' := (fun l => (l, n)) <$> predecessors m zxg in
+  let succs' := (fun r => (n, r)) <$> successors m zxg in
+  let preds'' := (fun l => (l, n)) <$> predecessors n zxg in
+  let succs'' := (fun r => (n, r)) <$> successors n zxg in 
+  let rot_n : option R := rotation n zxg in
+  let rot_m : option R := rotation m zxg in
+  if option_eqb_bool (vertex_type n zxg) (vertex_type m zxg) then 
+    match rot_n with
+    | Some r1 => 
+      match rot_m with
+      | Some r2 => add_vertex n (true, (r1 + r2)%R) 
+        (add_edges (preds' ++ preds'' ++ succs' ++ succs'') (remove_vertex n (remove_vertex m zxg)))
+      | None => zxg
+      end
+    | None => zxg
+    end
+    else
+      zxg.
